crates/move-stackless-bytecode/src/stackless_bytecode.rs
@@ -147,6 +147,7 @@ pub enum QuantifierHelperType {
     FindIndex,
     FindIndices,
     Filter,
+    Count,
 }
 
 impl QuantifierHelperType {
@@ -157,6 +158,7 @@ impl QuantifierHelperType {
             QuantifierHelperType::FindIndex => "find_index",
             QuantifierHelperType::FindIndices => "find_indices",
             QuantifierHelperType::Filter => "filter",
+            QuantifierHelperType::Count => "count",
         }
     }
 }
@@ -248,10 +250,10 @@ impl QuantifierType {
             | QuantifierType::FindIndexRange
             | QuantifierType::Find
             | QuantifierType::FindRange => Some(QuantifierHelperType::FindIndex),
-            QuantifierType::FindIndices
-            | QuantifierType::FindIndicesRange
-            | QuantifierType::Count
-            | QuantifierType::CountRange => Some(QuantifierHelperType::FindIndices),
+            QuantifierType::FindIndices | QuantifierType::FindIndicesRange => {
+                Some(QuantifierHelperType::FindIndices)
+            }
+            QuantifierType::Count | QuantifierType::CountRange => Some(QuantifierHelperType::Count),
             QuantifierType::Filter | QuantifierType::FilterRange => {
                 Some(QuantifierHelperType::Filter)
             }
